theories/hazptr/code_treiber.v
@@ -59,3 +59,6 @@ Definition tstack_pop : val :=
     "ov".
 
 End treiber.
+
+
+Check tstack_pop_loop.
